Refinery/Term/Extrinsic/Wk.lean
@@ -1,8 +1,18 @@
-import Refinery.Term.Syntax
+import Refinery.Term.Extrinsic.Typing
 import Refinery.Ctx.Basic
 
 namespace Refinery
 
 namespace Term
 
-variable {α : Type v} {ε : Type w} [HasQuant α] [PartialOrder ε]
+variable {φ : Type u} {α : Type v} {ε : Type w} [S : Signature φ α ε]
+
+def Deriv.wk {e : ε} {Γ Δ : Ctx? α ε} (ρ : Γ.Wk Δ) {A : Ty α} {a : Term φ}
+  : (Δ ⊢[e] a : A) → (Γ ⊢[e] a.ren ρ : A)
+  | .bv hv => .bv (hv.wkIn ρ)
+  | .op hf da => .op hf (da.wk ρ)
+  | _ => sorry
+
+end Term
+
+end Refinery
