Refinery.lean
@@ -1,3 +1,3 @@
 import Refinery.Ty
 import Refinery.Term
-import Refinery.Term.Extrinsic.Semantics
+import Refinery.Term.Extrinsic.Semantics.Typing
